theories/Template/QuoteGround/Environment.v
@@ -27,35 +27,38 @@ Module Type QuoteTerm (T : Term).
 End QuoteTerm.
 
 Module Type QuotationOfEnvironment (T : Term) (Import E : EnvironmentSig T).
-  #[export] Declare Instance qBuild_constructor_body : quotation_of Build_constructor_body.
-  #[export] Declare Instance qBuild_projection_body : quotation_of Build_projection_body.
+  #[export] Declare Instance qconstructor_body : inductive_quotation_of constructor_body.
+  #[export] Declare Instance qprojection_body : inductive_quotation_of projection_body.
+  #[export] Declare Instance qone_inductive_body : inductive_quotation_of one_inductive_body.
+  #[export] Declare Instance qmutual_inductive_body : inductive_quotation_of mutual_inductive_body.
+  #[export] Declare Instance qconstant_body : inductive_quotation_of constant_body.
+  #[export] Declare Instance qglobal_decl : inductive_quotation_of global_decl.
+  #[export] Declare Instance qglobal_env : inductive_quotation_of global_env.
+  #[export] Declare Instance qAll_decls : inductive_quotation_of All_decls.
+  #[export] Declare Instance qAll_decls_alpha : inductive_quotation_of All_decls_alpha.
 End QuotationOfEnvironment.
 
 Module QuoteEnvironment (T : Term) (Import E : EnvironmentSig T) (Import QT : QuoteTerm T) (Import QoE : QuotationOfEnvironment T E).
 
   #[export] Instance quote_constructor_body : ground_quotable constructor_body := ltac:(destruct 1; exact _).
-    #[export] Instance quote_projection_body : ground_quotable projection_body := ltac:(destruct 1; exact _).
-    #[export] Instance quote_one_inductive_body : ground_quotable one_inductive_body := ltac:(destruct 1; exact _).
-    #[export] Instance quote_mutual_inductive_body : ground_quotable mutual_inductive_body := ltac:(destruct 1; exact _).
-    #[export] Instance quote_constant_body : ground_quotable constant_body := ltac:(destruct 1; exact _).
-    #[export] Instance quote_global_decl : ground_quotable global_decl := ltac:(destruct 1; exact _).
-    #[export] Instance quote_global_env : ground_quotable global_env := ltac:(destruct 1; exact _).
+  #[export] Instance quote_projection_body : ground_quotable projection_body := ltac:(destruct 1; exact _).
+  #[export] Instance quote_one_inductive_body : ground_quotable one_inductive_body := ltac:(destruct 1; exact _).
+  #[export] Instance quote_mutual_inductive_body : ground_quotable mutual_inductive_body := ltac:(destruct 1; exact _).
+  #[export] Instance quote_constant_body : ground_quotable constant_body := ltac:(destruct 1; exact _).
+  #[export] Instance quote_global_decl : ground_quotable global_decl := ltac:(destruct 1; exact _).
 
+  #[export] Instance quote_global_env : ground_quotable global_env := ltac:(destruct 1; exact _).
+
+  #[export] Instance qcst_type : quotation_of cst_type := ltac:(cbv -[quotation_of]; exact _).
+  #[export] Instance qcst_body : quotation_of cst_body := ltac:(cbv -[quotation_of]; exact _).
+  #[export] Instance qcst_universes : quotation_of cst_universes := ltac:(cbv -[quotation_of]; exact _).
+  #[export] Instance quniverses : quotation_of universes := ltac:(cbv -[quotation_of]; exact _).
   #[export] Instance qdeclarations : quotation_of declarations := ltac:(cbv -[quotation_of]; exact _).
-  Import Template.utils.bytestring.
-  Print qdeclarations.
-  Section with_quote.
-    Context {qglobal_decl : quotation_of global_decl}.
+  #[export] Instance qglobal_declarations : quotation_of global_declarations := ltac:(cbv [global_declarations]; exact _).
 
-    #[export] Instance qcst_type : quotation_of cst_type := ltac:(cbv -[quotation_of]; exact _).
-    #[export] Instance qcst_body : quotation_of cst_body := ltac:(cbv -[quotation_of]; exact _).
-    #[export] Instance qcst_universes : quotation_of cst_universes := ltac:(cbv -[quotation_of]; exact _).
-
-    #[export] Instance qglobal_declarations : quotation_of global_declarations := ltac:(cbv [global_declarations]; exact _).
-    #[export] Instance quote_extends {Σ Σ'} : ground_quotable (@extends Σ Σ') := ltac:(cbv [extends]; exact _).
-    #[export] Instance quote_extends_decls {Σ Σ'} : ground_quotable (@extends_decls Σ Σ') := ltac:(cbv [extends_decls]; exact _).
-    #[export] Instance quote_primitive_invariants {cdecl} : ground_quotable (primitive_invariants cdecl) := _.
-  End with_quote.
+  #[export] Instance quote_extends {Σ Σ'} : ground_quotable (@extends Σ Σ') := ltac:(cbv [extends]; exact _).
+  #[export] Instance quote_extends_decls {Σ Σ'} : ground_quotable (@extends_decls Σ Σ') := ltac:(cbv [extends_decls]; exact _).
+  #[export] Instance quote_primitive_invariants {cdecl} : ground_quotable (primitive_invariants cdecl) := _.
 
   #[export] Instance quote_All_decls {P t t'} {qP : quotation_of P} {quoteP : forall t t', ground_quotable (P t t')} : ground_quotable (All_decls P t t') := ltac:(induction 1; exact _).
   #[export] Instance quote_All_decls_alpha {P t t'} {qP : quotation_of P} {quoteP : forall t t', ground_quotable (P t t')} : ground_quotable (All_decls_alpha P t t') := ltac:(induction 1; exact _).
@@ -69,6 +72,11 @@ Module QuoteEnvironment (T : Term) (Import E : EnvironmentSig T) (Import QT : Qu
      quote_constant_body
      quote_global_decl
      quote_global_env
+     qcst_type
+     qcst_body
+     qcst_universes
+     quniverses
+     qdeclarations
      qglobal_declarations
      quote_extends
      quote_extends_decls
